common/Values.v
@@ -29,13 +29,13 @@ Parameter eq_block : forall (x y:block),{x=y}+{x<>y}.
 
 End BLOCK.
 
-Declare Module Block : BLOCK.
-(*
+(* Declare Module Block : BLOCK. *)
+
 Module Block <: BLOCK.
 Definition block := positive.
 Definition eq_block := peq.
 End Block.
-*)
+
 Definition block := Block.block.
 Definition eq_block := Block.eq_block.
 
